Progress on proving correctness of last compilation step.

deps/poulet4/lib/P4automata/CompileFirstOrderConfRelSimplified.v
@@ -7,6 +7,7 @@ Require Import Poulet4.P4automata.ConfRel.
 Require Import Poulet4.P4automata.P4automaton.
 Require Import Poulet4.P4automata.Ntuple.
 Require Import Poulet4.P4automata.FirstOrder.
+Require Import Coq.Logic.JMeq.
 Import HListNotations.
 
 Require Poulet4.P4automata.FirstOrderConfRelSimplified.
@@ -40,28 +41,20 @@ Section CompileFirstOrderConfRelSimplified.
       CSnoc _ (compile_store_ctx_partial hdrs) (FOBV.Bits (projT1 hdr))
   }.
 
-  (* TODO: make this a normal fixpoint or equations definition *)
-  Definition compile_store_valu_partial
-    (hdrs: list (Syntax.H' H))
-    : (HList.t (fun x => (n_tuple bool (projT1 x))) hdrs)
-    -> valu FOBV.sig FOBV.fm_model (compile_store_ctx_partial hdrs).
-  refine ((
-    fix recur hdrs :=
-      match hdrs with 
-      | nil => fun _ => _
-      | hdr :: hdrs => fun vs => 
-        _
-      end 
-  ) hdrs).
-  - exact (VEmp _ _).
-  - inversion vs.
-    refine (VSnoc _ _ _ _ _ _).
-    + exact X.
-    + eapply recur. exact X0.
-  Defined.
-
   Definition compile_store_ctx : ctx FOBV.sig :=
     compile_store_ctx_partial (enum (Syntax.H' H)).
+
+  Equations compile_store_valu_partial
+    {hdrs: list (Syntax.H' H)}
+    (hl: HList.t (fun x => (n_tuple bool (projT1 x))) hdrs)
+    : valu FOBV.sig FOBV.fm_model (compile_store_ctx_partial hdrs)
+      by struct hl
+  := {
+    compile_store_valu_partial hnil := VEmp _ _;
+    compile_store_valu_partial (hdr ::: hdrs) :=
+      VSnoc _ FOBV.fm_model (FOBV.Bits _) _ hdr
+            (compile_store_valu_partial hdrs)
+  }.
 
   Equations compile_ctx (c: ctx (FOS.sig H)) : ctx FOBV.sig := {
     compile_ctx (CEmp _) := CEmp _;
@@ -71,34 +64,28 @@ Section CompileFirstOrderConfRelSimplified.
       CSnoc _ (compile_ctx c) (FOBV.Bits n)
   }.
 
-  Equations build_hlist_env 
+  Equations build_hlist_env
     (hdrs: list (Syntax.H' H))
     (env: P4A.store H)
     : (HList.t (fun x => (n_tuple bool (projT1 x))) hdrs) := {
       build_hlist_env nil _ := hnil;
-      build_hlist_env (hdr :: hdrs) env := 
-        _ ::: (build_hlist_env hdrs) env
+      build_hlist_env (hdr :: hdrs) env :=
+        let v := match P4A.find H (projT2 hdr) env with
+                 | P4A.VBits _ v => v
+                 end in
+        (_ v) ::: build_hlist_env hdrs env
     }.
-  Next Obligation.
-  exact (
-    match P4A.find H (projT2 hdr) env with 
-    | P4A.VBits _ v => v 
-    end
-  ).
-  Defined.
 
-  Equations compile_valu 
-    {c: ctx (FOS.sig H)} 
-    (v: valu (FOS.sig H) (FOS.fm_model a) c) 
+  Equations compile_valu
+    {c: ctx (FOS.sig H)}
+    (v: valu (FOS.sig H) (FOS.fm_model a) c)
     : valu FOBV.sig FOBV.fm_model (compile_ctx c) := {
     compile_valu (VEmp _ _) := VEmp _ _;
-    compile_valu (VSnoc _ _ (FOS.Bits n) _ v vinner) := 
+    compile_valu (VSnoc _ _ (FOS.Bits n) _ v vinner) :=
       VSnoc _ FOBV.fm_model (FOBV.Bits n) _ v (compile_valu vinner);
-    compile_valu (VSnoc _ _ (FOS.Store) _ v vinner) := 
-      app_valu _ (compile_valu vinner) (compile_store_valu_partial (build_hlist_env _ _))
+    compile_valu (VSnoc _ _ (FOS.Store) _ v vinner) :=
+      app_valu _ (compile_valu vinner) (compile_store_valu_partial (build_hlist_env _ v))
   }.
-  Next Obligation.
-  Defined.
 
   Lemma here_or_there
     {X: Type}
@@ -118,43 +105,31 @@ Section CompileFirstOrderConfRelSimplified.
       + exact H1.
   Defined.
 
-  Equations compile_lookup'
+  Equations compile_lookup_partial
     (k: Syntax.H' H)
     (enum: list (Syntax.H' H))
     (elem_of_enum: List.In k enum)
     : var (FOBV.sig) (compile_store_ctx_partial enum)
           (FOBV.Bits (projT1 k)) := {
-    compile_lookup' k (elem :: enum) elem_of_enum :=
+    compile_lookup_partial k (elem :: enum) elem_of_enum :=
       match here_or_there elem_of_enum with
-      | left Heq => eq_rec_r _ (fun _ =>
-          VHere _ (compile_store_ctx_partial enum) (FOBV.Bits (projT1 k))
-        ) Heq elem_of_enum
-      | right Helse => VThere FOBV.sig _ (FOBV.Bits (projT1 elem))
-                              _ (compile_lookup' k enum Helse)
+      | left Heq =>
+        _ (VHere _ (compile_store_ctx_partial enum) (FOBV.Bits (projT1 k)))
+      | right Helse =>
+        VThere FOBV.sig _ (FOBV.Bits (projT1 elem))
+               _ (compile_lookup_partial k enum Helse)
       end
   }.
 
   Definition compile_lookup (k: Syntax.H' H)
     : var FOBV.sig compile_store_ctx (FOBV.Bits (projT1 k))
   :=
-    compile_lookup' k (enum (Syntax.H' H)) (elem_of_enum k).
+    compile_lookup_partial k (enum (Syntax.H' H)) (elem_of_enum k).
 
-  Equations tm_cons {c s' s}
-    (t: tm FOBV.sig c s)
-    : tm FOBV.sig (CSnoc _ c s') s := {
-    tm_cons (TVar v) := TVar (VThere _ _ _ _ v);
-    tm_cons (TFun _ fn args) := TFun _ fn (tms_cons args)
-  } where tms_cons {c s' s}
-    (ts: HList.t (tm FOBV.sig c) s)
-    : HList.t (tm FOBV.sig (CSnoc _ c s')) s := {
-    tms_cons hnil := hnil;
-    tms_cons (t ::: ts) := tm_cons t ::: tms_cons ts
+  Equations compile_sizes (enum: list (Syntax.H' H)): nat := {
+    compile_sizes nil := 0;
+    compile_sizes (elem :: enum) := projT1 elem + compile_sizes enum;
   }.
-
-  Definition compile_sizes (enum: list (Syntax.H' H)): nat :=
-    let sizes := List.map (@projT1 nat H) enum in
-    (* let sizes' := List.filter (fun n => (0 <? n)%nat) sizes in  *)
-    List.fold_right Nat.add 0 sizes.
 
   Definition compile_sort (s: FOS.sorts) : FOBV.sorts :=
     match s with
@@ -162,21 +137,21 @@ Section CompileFirstOrderConfRelSimplified.
     | FOS.Store => FOBV.Bits (compile_sizes (enum (Syntax.H' H)))
     end.
 
-  Equations compile_store'
+  Equations compile_store_partial
     (enum: list (Syntax.H' H))
     : tm FOBV.sig (compile_store_ctx_partial enum)
                   (FOBV.Bits (compile_sizes enum)) := {
-    compile_store' nil := TFun FOBV.sig (FOBV.BitsLit 0 tt) hnil;
-    compile_store' (elem :: enum) :=
+    compile_store_partial nil := TFun FOBV.sig (FOBV.BitsLit 0 tt) hnil;
+    compile_store_partial (elem :: enum) :=
       TFun FOBV.sig (FOBV.Concat (projT1 elem) (compile_sizes enum))
                     (TVar (VHere _ _ _) :::
-                     tm_cons (compile_store' enum) ::: hnil)
+                     tm_cons FOBV.sig (compile_store_partial enum) ::: hnil)
   }.
 
   Definition compile_store
     : tm (FOBV.sig) compile_store_ctx (compile_sort FOS.Store)
   :=
-    compile_store' (enum (Syntax.H' H)).
+    compile_store_partial (enum (Syntax.H' H)).
 
   Equations subscript {c n}
     (v: var (FOS.sig H) c FOS.Store)
@@ -200,7 +175,7 @@ Section CompileFirstOrderConfRelSimplified.
     compile_var (VHere _ c (FOS.Bits n)) :=
       TVar (VHere _ (compile_ctx c) (FOBV.Bits n));
     compile_var (VHere _ c FOS.Store) := reindex_tm compile_store;
-    compile_var (VThere _ c (FOS.Bits _) s' v) := tm_cons (compile_var v);
+    compile_var (VThere _ c (FOS.Bits _) s' v) := tm_cons FOBV.sig (compile_var v);
     compile_var (VThere _ c FOS.Store s' v) := weaken_tm _ (compile_var v)
   }.
 
@@ -238,39 +213,398 @@ Section CompileFirstOrderConfRelSimplified.
       quantify compile_store_ctx (compile_fm f)
   }.
 
-  
+  Equations compile_store_val_partial
+    (s: store (P4A.interp a))
+    (enum: list (Syntax.H' H))
+    : n_tuple bool (compile_sizes enum)
+  := {
+    compile_store_val_partial s nil := tt;
+    compile_store_val_partial s (elem :: enum) :=
+      let '(P4A.VBits _ v) := P4A.find H (projT2 elem) s in
+      n_tuple_concat v (compile_store_val_partial s enum)
+  }.
 
-  
+  Equations compile_val
+    {sort: FOS.sorts}
+    (val: FOS.mod_sorts a sort)
+    : FOBV.mod_sorts (compile_sort sort)
+  := {
+    @compile_val (FOS.Bits _) v := _ v;
+    @compile_val FOS.Store s :=
+      compile_store_val_partial s (enum (Syntax.H' H));
+  }.
+
+  Lemma compile_store_val_correct:
+    forall (n: nat) (h : H n) c (v0 : var (FOS.sig H) c FOS.Store) v,
+      compile_val (sort := FOS.Bits n)
+        match P4A.find H h (find (FOS.sig H) (FOS.fm_model a) v0 v)
+        with
+        | P4A.VBits _ v1 => v1
+        end =
+      find FOBV.sig FOBV.fm_model
+        (subscript v0 (compile_lookup (existT H n h))) (compile_valu v).
+  Proof.
+  Admitted.
+
+  Equations decompile_store_val_partial
+    (enum: list (Syntax.H' H))
+    (val: n_tuple bool (compile_sizes enum))
+    : store (P4A.interp a)
+  := {
+    decompile_store_val_partial nil val := nil;
+    decompile_store_val_partial (elem :: enum) val :=
+      let prefix := rewrite_size _ (n_tuple_take_n (projT1 elem) val) in
+      let suffix := rewrite_size _ (n_tuple_skip_n (projT1 elem) val) in
+      P4A.assign H (projT2 elem) (P4A.VBits _ prefix)
+                   (decompile_store_val_partial enum suffix)
+  }.
+  Next Obligation.
+    autorewrite with compile_sizes; Lia.lia.
+  Defined.
+  Next Obligation.
+    autorewrite with compile_sizes; Lia.lia.
+  Defined.
+
+  Equations decompile_val
+    {sort: FOS.sorts}
+    (val: FOBV.mod_sorts (compile_sort sort))
+    : FOS.mod_sorts a sort
+  := {
+    @decompile_val (FOS.Bits _) v := v;
+    @decompile_val FOS.Store v :=
+      decompile_store_val_partial (enum (Syntax.H' H)) v;
+  }.
+
+  Lemma compile_store_val_partial_invariant:
+    forall h v enum s,
+      ~ List.In h enum ->
+      compile_store_val_partial (P4A.assign H (projT2 h) v s) enum =
+      compile_store_val_partial s enum.
+  Proof.
+    intros.
+    induction enum.
+    - reflexivity.
+    - autorewrite with compile_store_val_partial; simpl.
+      rewrite IHenum.
+      + rewrite P4A.find_not_first; auto.
+        contradict H0.
+        subst; now apply List.in_eq.
+      + contradict H0.
+        now apply List.in_cons.
+  Qed.
+
+  Lemma decompile_store_val_partial_roundtrip:
+    forall enum val,
+      List.NoDup enum ->
+      val ~= compile_store_val_partial (decompile_store_val_partial enum val) enum.
+  Proof.
+    induction enum; intros.
+    - autorewrite with decompile_store_val_partial.
+      autorewrite with compile_store_val_partial.
+      now destruct val.
+    - autorewrite with decompile_store_val_partial.
+      autorewrite with compile_store_val_partial.
+      simpl.
+      rewrite P4A.assign_find.
+      symmetry.
+      rewrite <- NtupleProofs.n_tuple_concat_roundtrip with (n := projT1 a0).
+      symmetry.
+      apply NtupleProofs.concat_proper with
+        (xs2 := (rewrite_size (decompile_store_val_partial_obligations_obligation_1 a0 enum) _))
+        (ys2 := (compile_store_val_partial _ enum)).
+      + now rewrite rewrite_size_jmeq.
+      + inversion H0.
+        now rewrite compile_store_val_partial_invariant,
+                    <- IHenum,
+                    rewrite_size_jmeq by auto.
+  Qed.
+
+  Lemma compile_val_roundtrip:
+    forall s (val: FOBV.mod_sorts (compile_sort s)),
+      val = compile_val (decompile_val val).
+  Proof.
+    intros.
+    destruct s.
+    - reflexivity.
+    - autorewrite with decompile_val.
+      autorewrite with compile_val.
+      rewrite <- decompile_store_val_partial_roundtrip; auto.
+      apply NoDup_enum.
+  Qed.
+
+  Inductive val_almost_equal:
+    forall s,
+      FOS.mod_sorts a s ->
+      FOS.mod_sorts a s ->
+      Prop
+  :=
+  | ValAlmostEqualBits:
+      forall (n: nat) (t: n_tuple bool n), val_almost_equal (FOS.Bits n) t t
+  | ValAmostEqualStore:
+      forall (s1 s2: store (P4A.interp a)),
+        (forall n (h: H n), P4A.find H h s1 = P4A.find H h s2) ->
+        val_almost_equal FOS.Store s1 s2.
+
+  Definition store_almost_equal (s1 s2: store (P4A.interp a)) :=
+    forall n (h: H n), P4A.find H h s1 = P4A.find H h s2.
+
+  Axiom store_eq:
+    forall (s1 s2: store (P4A.interp a)),
+      store_almost_equal s1 s2 ->
+      s1 = s2.
+
+  Lemma decompile_val_roundtrip:
+    forall s (val: FOS.mod_sorts a s),
+      val = decompile_val (compile_val val).
+  Proof.
+    intros.
+    destruct s.
+    - autorewrite with compile_val.
+      autorewrite with decompile_val.
+      constructor.
+    - apply store_eq.
+      unfold store_almost_equal; intros.
+      autorewrite with compile_val.
+      autorewrite with decompile_val.
+      pose proof (elem_of_enum (Finite := H_finite) (existT _ n h)).
+      revert h H0; induction (enum (Syntax.H' H)); intros.
+      + contradiction.
+      + destruct (existT _ n h == a0).
+        * unfold equiv in e.
+          subst.
+          clear IHl.
+          autorewrite with compile_store_val_partial.
+          autorewrite with decompile_store_val_partial.
+          simpl.
+          rewrite P4A.assign_find.
+          destruct (P4A.find H h val).
+          f_equal.
+          apply JMeq_eq.
+          rewrite rewrite_size_jmeq.
+          pose proof NtupleProofs.n_tuple_take_n_roundtrip.
+          now specialize (H1 n n0 _ (compile_store_val_partial val l)).
+        * unfold equiv, complement in c.
+          autorewrite with compile_store_val_partial.
+          autorewrite with decompile_store_val_partial.
+          simpl.
+          replace h with (projT2 (existT _ n h)).
+          pose proof P4A.find_not_first.
+          specialize (H1 H _ _ (existT H n h) a0).
+          rewrite H1.
+          rewrite IHl.
+          f_equal.
+          f_equal.
+          destruct (P4A.find H (projT2 a0) val).
+          apply JMeq_eq.
+          rewrite rewrite_size_jmeq.
+          pose proof NtupleProofs.n_tuple_skip_n_roundtrip.
+          now specialize (H2 (projT1 a0) n0 _ (compile_store_val_partial val l)).
+          simpl.
+          destruct H0.
+          congruence.
+          assumption.
+          easy.
+          now simpl.
+  Qed.
+
+  Lemma compile_store_val_partial_correct':
+    forall enum m,
+      compile_store_val_partial m enum =
+      interp_tm
+          (compile_store_valu_partial (build_hlist_env enum m))
+          (compile_store_partial enum).
+  Proof.
+    induction enum; intros.
+    - reflexivity.
+    - autorewrite with compile_store_val_partial.
+      autorewrite with build_hlist_env.
+      simpl.
+      unfold build_hlist_env_obligations_obligation_1.
+      destruct (P4A.find H (projT2 a0) m).
+      rewrite (compile_store_valu_partial_equation_2 a0 (rest := enum) n).
+      rewrite (compile_store_partial_equation_2 a0 enum).
+      autorewrite with interp_tm; simpl.
+      autorewrite with mod_fns.
+      f_equal.
+      rewrite <- interp_tm_tm_cons.
+      apply IHenum.
+  Qed.
+
+  Lemma compile_store_val_partial_correct:
+    forall m,
+      compile_store_val_partial m (enum (Syntax.H' H)) =
+      interp_tm
+          (compile_store_valu_partial (build_hlist_env (enum (Syntax.H' H)) m))
+          (compile_store_partial (enum (Syntax.H' H))).
+  Proof.
+    apply compile_store_val_partial_correct'.
+  Qed.
+
+  Lemma compile_var_correct:
+    forall c s (v: var _ c s) val,
+      compile_val (interp_tm (m := FOS.fm_model a) val (TVar v)) =
+      interp_tm (compile_valu val) (compile_var v).
+  Proof.
+    dependent induction val; intros.
+    - dependent destruction v.
+    - dependent destruction v.
+      + destruct s; [easy|].
+        rewrite (compile_var_equation_2 c).
+        rewrite (compile_valu_equation_3 (c0 := c) m).
+        unfold compile_store.
+        autorewrite with interp_tm.
+        autorewrite with find.
+        replace (@interp_tm FOBV.sig FOBV.fm_model _ _ _ _)
+        with (interp_tm
+                (compile_store_valu_partial (build_hlist_env (enum (Syntax.H' H)) m))
+                (compile_store_partial (enum (Finite := H_finite) (Syntax.H' H)))).
+        * autorewrite with compile_val.
+          apply compile_store_val_partial_correct.
+        * now rewrite interp_tm_reindex_tm with (sig := FOBV.sig) (v' := compile_valu val).
+      + destruct s0.
+        * rewrite (compile_var_equation_3 n (ctx1 := c)).
+          rewrite (compile_valu_equation_2 (c0 := c) n).
+          replace (@interp_tm FOBV.sig FOBV.fm_model _ _ _ _)
+          with (interp_tm (compile_valu val) (compile_var v)).
+          autorewrite with interp_tm.
+          autorewrite with find.
+          rewrite <- IHval.
+          now autorewrite with interp_tm.
+          now rewrite interp_tm_tm_cons with
+            (sig := FOBV.sig)
+            (m := FOBV.fm_model)
+            (s' := FOBV.Bits n)
+            (val := m).
+        * rewrite (compile_var_equation_4 v).
+          rewrite (compile_valu_equation_3 (c0 := c) m).
+          autorewrite with interp_tm.
+          autorewrite with find.
+          replace (@interp_tm FOBV.sig FOBV.fm_model _ _ _ _)
+          with (interp_tm (compile_valu val) (compile_var v)).
+          rewrite <- IHval.
+          -- now autorewrite with interp_tm.
+          -- now rewrite interp_tm_weaken_tm with
+               (v' := (compile_store_valu_partial (build_hlist_env (enum (Syntax.H' H)) m))).
+  Qed.
+
+  Lemma compile_simplified_tm_bv_correct:
+    forall c s v (tm: tm _ c s),
+      compile_val (interp_tm (m := FOS.fm_model a) v tm) =
+      interp_tm (compile_valu v) (compile_tm (c := c) tm).
+  Proof.
+    intros.
+    dependent induction tm using tm_ind'.
+    - autorewrite with compile_tm.
+      apply compile_var_correct.
+    - destruct srt;
+      repeat dependent destruction hl;
+      autorewrite with compile_tm;
+      autorewrite with interp_tm; simpl;
+      autorewrite with mod_fns;
+      repeat match goal with
+      | H : HList.all _ _ |- _ =>
+        destruct H
+      end;
+      auto.
+      + unfold compile_val_obligations_obligation_1.
+        now rewrite <- H0, <- H1.
+      + now rewrite <- H0.
+      + dependent destruction t; [|easy].
+        autorewrite with compile_tm.
+        autorewrite with interp_tm.
+        apply compile_store_val_correct.
+  Qed.
+
+  Lemma compile_store_valu_partial_invariant:
+    forall h v enum s,
+      ~ List.In h enum ->
+      compile_store_valu_partial (build_hlist_env enum (P4A.assign H (projT2 h) v s)) =
+      compile_store_valu_partial (build_hlist_env enum s).
+  Proof.
+    (* Probably something similar to compile_store_val_partial_invariant *)
+  Admitted.
+
+  Lemma compile_store_valu_partial_surjective':
+    forall enum,
+      List.NoDup enum ->
+      forall (val: valu FOBV.sig FOBV.fm_model (compile_store_ctx_partial enum)),
+        exists s: P4A.store H,
+          compile_store_valu_partial (build_hlist_env enum s) = val.
+  Proof.
+    induction enum; intros.
+    - exists nil.
+      autorewrite with build_hlist_env.
+      dependent destruction val.
+      now rewrite <- compile_store_valu_partial_equation_1.
+    - dependent destruction val.
+      inversion H0.
+      specialize (IHenum H4 val).
+      destruct IHenum as [? ?].
+      exists (P4A.assign H (projT2 a0) (P4A.VBits _ m) x0).
+      autorewrite with build_hlist_env.
+      simpl.
+      unfold build_hlist_env_obligations_obligation_1.
+      rewrite P4A.assign_find.
+      rewrite (compile_store_valu_partial_equation_2 a0 (rest := enum) m).
+      f_equal.
+      now rewrite compile_store_valu_partial_invariant.
+  Qed.
+
+  Lemma compile_store_valu_partial_surjective:
+    forall (val: valu FOBV.sig FOBV.fm_model compile_store_ctx),
+      exists s: P4A.store H,
+        compile_store_valu_partial (build_hlist_env (enum (Syntax.H' H)) s) = val.
+  Proof.
+    intros.
+    apply compile_store_valu_partial_surjective'.
+    apply NoDup_enum.
+  Qed.
 
   Lemma compile_simplified_fm_bv_correct:
-      forall c v (fm : fm _ c),
-        interp_fm (m := FOS.fm_model a) v fm <->
-        interp_fm (m := FOBV.fm_model) (compile_valu v) (compile_fm (c := c) fm)
-        .
+    forall c v (fm : fm _ c),
+      interp_fm (m := FOS.fm_model a) v fm <->
+      interp_fm (m := FOBV.fm_model) (compile_valu v) (compile_fm (c := c) fm)
+      .
   Proof.
     intros.
     dependent induction fm;
     autorewrite with compile_fm;
     autorewrite with interp_fm;
-    try (
-      (now (split; intros; trivial)) ||
-      now (setoid_rewrite IHfm; apply iff_refl) || 
-      now (setoid_rewrite IHfm1; setoid_rewrite IHfm2; apply iff_refl)
-    ).
-
-    - admit.
-    - setoid_rewrite IHfm.
-      split;
-      intros.
+    try easy.
+    - repeat rewrite <- compile_simplified_tm_bv_correct.
+      split; intros.
+      + now f_equal.
+      + rewrite decompile_val_roundtrip.
+        rewrite decompile_val_roundtrip at 1.
+        now f_equal.
+    - now rewrite IHfm.
+    - now rewrite IHfm1, IHfm2.
+    - now rewrite IHfm1, IHfm2.
+    - now rewrite IHfm1, IHfm2.
+    - destruct s.
       + autorewrite with compile_fm.
-        destruct s; autorewrite with compile_fm.
-        * autorewrite with interp_fm.
-          eapply H0.
-        * unfold compile_store_ctx.
-          admit.
-      + admit.
-  
-  Admitted.
+        autorewrite with interp_fm.
+        intuition.
+        -- specialize (H0 (decompile_val val (sort := FOS.Bits n))).
+           apply IHfm in H0.
+           apply H0.
+        -- specialize (H0 (compile_val val)).
+           apply IHfm.
+           apply H0.
+      + autorewrite with compile_fm.
+        rewrite quantify_correct.
+        intuition.
+        -- pose proof (compile_store_valu_partial_surjective valu).
+           destruct H1 as [s ?].
+           specialize (H0 s).
+           apply IHfm in H0.
+           rewrite (compile_valu_equation_3 s (c0 := c)) in H0.
+           now rewrite H1 in H0.
+        -- specialize (H0 (compile_store_valu_partial (build_hlist_env _ val))).
+           apply IHfm.
+           now rewrite (compile_valu_equation_3 val (c0 := c)).
+  Qed.
+
 End CompileFirstOrderConfRelSimplified.
 
 Register FOBV.Bits as p4a.sorts.bits.
