deps/poulet4/lib/P4automata/DepEnv.v
@@ -3,25 +3,25 @@ Import List.ListNotations.
 
 Section DepEnv.
   Variable (I: Type).
-  Context `{I_eq_dec: EquivDec.EqDec I eq}.
   Variable (K: I -> Type).
-  Context `{K_eq_dec: forall i, EquivDec.EqDec (K i) eq}.
   Variable (V: I -> Type).
 
   Definition binding :=
     {i: I & K i & V i}.
+  Definition key :=
+    {i: I & K i}.
+
+  Context `{K_eq_dec: EquivDec.EqDec key eq}.
 
   Definition t := list binding.
 
   Fixpoint find {i} (k: K i) (e: t) : option (V i).
+  Proof.
     destruct e as [ | [j k' v] e'].
     - exact None.
-    - destruct (i == j).
-      + unfold "===" in e.
-        subst j.
-        destruct (k == k').
-        * exact (Some v).
-        * exact (find i k e').
+    - destruct (existT K i k == existT K j k').
+      + inversion e; subst.
+        exact (Some v).
       + exact (find i k e').
   Defined.
 
