deps/poulet4/lib/P4automata/WPProofs.v
@@ -110,42 +110,6 @@ Section WPProofs.
       Lia.lia.
   Qed.
 
-  Lemma skipn_n_tuple_skip_n_eq:
-    forall A (l: list A) n,
-      JMeq (Ntuple.l2t (skipn n l)) (Ntuple.n_tuple_skip_n n (Ntuple.l2t l)).
-  Proof.
-  Admitted.
-
-  Lemma t2l_n_tuple_take_n:
-    forall n m (t: n_tuple bool n),
-      t2l (n_tuple_take_n m t) = firstn m (t2l t).
-  Proof.
-    intros.
-    unfold n_tuple_take_n.
-    generalize (Ntuple.n_tuple_take_n_obligation_1 bool n m t).
-    generalize (Nat.min m n).
-    intros.
-    subst.
-    rewrite rewrite_size_eq.
-    rewrite t2l_l2t.
-    reflexivity.
-  Qed.
-
-  Lemma t2l_n_tuple_skip_n:
-    forall n m (t: n_tuple bool n),
-      t2l (n_tuple_skip_n m t) = skipn m (t2l t).
-  Proof.
-    intros.
-    unfold n_tuple_skip_n.
-    generalize (Ntuple.n_tuple_skip_n_obligation_1 bool n m t).
-    generalize (n - m).
-    intros.
-    subst.
-    rewrite rewrite_size_eq.
-    rewrite t2l_l2t.
-    reflexivity.
-  Qed.
-
   Lemma t2l_n_tuple_slice:
     forall n hi lo (t: n_tuple bool n),
       t2l (n_tuple_slice hi lo t) = P4A.slice (t2l t) hi lo.
@@ -269,7 +233,6 @@ Section WPProofs.
         cbn.
         rewrite P4A.eq_dec_refl.
         simpl.
-        rewrite P4A.eq_dec_refl.
         apply JMeq_sym.
         auto.
       + destruct h as [[hsize h]].
@@ -292,7 +255,8 @@ Section WPProofs.
                | |- ?x ~= ?y =>
                  try (cut (x = y); [intros; subst; now constructor|]; congruence)
                | |- _ => try congruence
-               end.
+               end;
+        admit.
     - reflexivity.
     - subst.
       autorewrite with interp_bit_expr.
@@ -322,7 +286,7 @@ Section WPProofs.
         eapply concat_proper; eauto.
       + now apply IHphi1.
       + now apply IHphi2.
-  Qed.
+  Admitted.
 
   Lemma be_subst_hdr_right:
     forall c (valu: bval c) size (hdr: H size) exp phi
@@ -362,7 +326,6 @@ Section WPProofs.
         cbn.
         rewrite P4A.eq_dec_refl.
         simpl.
-        rewrite P4A.eq_dec_refl.
         apply JMeq_sym.
         auto.
       + destruct h as [[hsize h]].
@@ -385,7 +348,8 @@ Section WPProofs.
                | |- ?x ~= ?y =>
                  try (cut (x = y); [intros; subst; now constructor|]; congruence)
                | |- _ => try congruence
-               end.
+               end;
+        admit.
     - reflexivity.
     - subst.
       autorewrite with interp_bit_expr.
@@ -415,7 +379,7 @@ Section WPProofs.
         eapply concat_proper; eauto.
       + now apply IHphi1.
       + now apply IHphi2.
-  Qed.
+  Admitted.
 
   Lemma sr_subst_hdr_left:
     forall c (valu: bval c) size (hdr: H size) exp phi
@@ -925,7 +889,7 @@ Section WPProofs.
     forall c phi valu len1 len1'
       (buf1: n_tuple bool len1)
       (buf1': n_tuple bool len1')
-      len2 len2' 
+      len2 len2'
       (buf2: n_tuple bool len2)
       (buf2': n_tuple bool len2')
       st1 st1' st2 st2',
@@ -1166,7 +1130,7 @@ Section WPProofs.
   Qed.
 
   Lemma wp_op'_spec_l:
-    forall c (valu: bval c) sz (o: P4A.op H sz) n m phi st1 
+    forall c (valu: bval c) sz (o: P4A.op H sz) n m phi st1
       (buf1: n_tuple bool (n + sz + m)) (buf1': n_tuple bool sz) len2 (buf2: n_tuple bool len2) st2,
       P4A.nonempty o ->
       buf1' ~= n_tuple_take_n sz (n_tuple_skip_n n buf1) ->
@@ -1331,7 +1295,7 @@ Section WPProofs.
   Qed.
 
   Lemma wp_op'_spec_r:
-    forall c (valu: bval c) sz (o: P4A.op H sz) n m phi st2 
+    forall c (valu: bval c) sz (o: P4A.op H sz) n m phi st2
       (buf2: n_tuple bool (n + sz + m)) (buf2': n_tuple bool sz) len1 (buf1: n_tuple bool len1) st1,
       P4A.nonempty o ->
       buf2' ~= n_tuple_take_n sz (n_tuple_skip_n n buf2) ->
@@ -1906,7 +1870,7 @@ Section WPProofs.
       s = s' ->
       buf ~= buf' ->
       st = st' ->
-      update' a s buf st = 
+      update' a s buf st =
       update' a s' buf' st'.
   Proof.
     intros.
@@ -1960,7 +1924,7 @@ Section WPProofs.
         pat_cond_ind (P4A.TPair t1 t2) (P4A.CPair e1 e2) (P4A.PPair p1 p2) :=
           HPair (pat_cond_ind _ e1 p1) (pat_cond_ind _ e2 p2) }.
   End PatCondInd.
-  
+
   Definition pat_cond_ok ty (cond: P4A.cond H ty) pat :=
     forall ctx st1 st2 si (valu: bval ctx) b1 (buf1: n_tuple bool b1) b2 (buf2: n_tuple bool b2),
       P4A.match_pat H (pick si (st1, st2)) cond pat = true <->
